src/ReactorModel/Determinism/State.lean
@@ -14,55 +14,32 @@ theorem exec_objₘ_rcn_eq {s : State} (m₁ : rcn ∈ s.rtr[.rcn]) (m₂ : rcn 
     s.rtr⟦m₁⟧ = (s.exec rcn').rtr⟦m₂⟧ :=
   Equivalent.objₘ_rcn_eq (s.exec_equiv rcn') m₁ |>.choose_spec
 
-
-
-
-
-theorem port_not_mem_indep_output {s : State} {k i} {rcn₁ rcn₂ : ID}
-    (hi : rcn₁ ≮[s.rtr] rcn₂) (m₂ : rcn₂ ∈ s.rtr[.rcn]) (hd : .port k i ∈ s.rtr⟦m₂⟧.deps .in) : 
-    (s.output rcn₁).All₂ (¬·.Targets (.prt k) i) := by
+theorem target_not_mem_indep_output {s : State} {i} {rcn₁ rcn₂ : ID}
+    (hi : rcn₁ ≮[s.rtr] rcn₂) (m₂ : rcn₂ ∈ s.rtr[.rcn]) (hd : ⟨cpt, i⟩ ∈ s.rtr⟦m₂⟧.deps .in) : 
+    (s.output rcn₁).All₂ (¬·.Targets cpt i) := by
   apply List.all₂_iff_forall.mpr
-  intro c hc ht
-  cases ht
+  intro c hc
   simp [output] at hc
-  split at hc
-  case inr => contradiction
+  split at hc <;> try contradiction
   case inl m₁ =>
+    intro ⟨⟩ 
     have := hi.deps_disjoint m₁ m₂
-    have := s.rtr⟦m₁⟧.prtOutDepOnly hc
+    have := s.rtr⟦m₁⟧.targetMemDeps hc
     exact Ne.irrefl $ Set.disjoint_iff_forall_ne.mp ‹_› ‹_› hd
 
-theorem exec_indep_input_ports_eq {s : State} {rcn₁ rcn₂ : ID} (hi : rcn₁ ≮[s.rtr] rcn₂) (m₁ m₂) :
-    input.ports (s.exec rcn₁) rcn₂ m₂ = input.ports s rcn₂ m₁ := by 
-  simp [input.ports]
-  ext1 k
+theorem exec_indep_restriction_eq {s : State} (hn : rcn₁ ≠ rcn₂) (hi : rcn₁ ≮[s.rtr] rcn₂) (m₁ m₂) : 
+    input.restriction (s.exec rcn₁) rcn₂ m₂ cpt = input.restriction s rcn₂ m₁ cpt := by 
+  simp [input.restriction]
   rw [←exec_objₘ_rcn_eq m₁ m₂]
-  exact Partial.ext_restrict 
-    fun _ hd => Reactor.apply'_preserves_unchanged $ port_not_mem_indep_output hi m₁ hd 
+  apply Partial.ext_restrict 
+  intro i hd
+  exact Reactor.apply'_preserves_unchanged $ target_not_mem_indep_output hi m₁ hd  
   
-
-
-
-set_option pp.proofs.withType false
-theorem exec_indep_input_state_eq {s : State} (hn : rcn₁ ≠ rcn₂) (hi : rcn₁ ≮[s.rtr] rcn₂) (m₁ m₂) : 
-    input.state (s.exec rcn₁) rcn₂ m₂ = input.state s rcn₂ m₁ := by 
-  simp [input.state, exec]
-  ext1 i
-  -- TODO: `s.output rcn₁` does not contain any changes to a state variable in `s.rtr⟦h✝⟧&`.
-  --       And hence not to i.
-  have H : (s.output rcn₁).All₂ (¬·.Targets .stv i) := sorry 
-  have G := s.rtr.apply'_preserves_unchanged H
-  sorry
-
-theorem exec_indep_input_acts_eq {s : State} (hn : rcn₁ ≠ rcn₂) (hi : rcn₁ ≮[s.rtr] rcn₂) (m₁ m₂) : 
-    input.acts (s.exec rcn₁) rcn₂ m₂ = input.acts s rcn₂ m₁ := by 
-  sorry
-
 theorem exec_indep_input_eq {s : State} (hn : rcn₁ ≠ rcn₂) (hi : rcn₁ ≮[s.rtr] rcn₂) : 
     (s.exec rcn₁).input rcn₂ = s.input rcn₂ := by 
   simp [input]
   split <;> split 
-  case inr.inr => rfl
+  case inr.inr => simp [exec]
   case inr.inl h => 
     have := Equivalent.mem_iff (Equivalent.symm $ Reactor.apply'_equiv _ $ s.output rcn₁) |>.mp h
     contradiction
@@ -70,97 +47,9 @@ theorem exec_indep_input_eq {s : State} (hn : rcn₁ ≠ rcn₂) (hi : rcn₁ �
     have := Equivalent.mem_iff (Reactor.apply'_equiv _ $ s.output rcn₁) |>.mp h
     contradiction
   case inl.inl m₂ m₁ =>
-    simp 
-    refine ⟨?ports, ?acts, ?state, rfl⟩
-    case state => apply exec_indep_input_state_eq ‹_› ‹_›   
-    case ports => apply exec_indep_input_ports_eq ‹_› ‹_›
-    case acts  => apply exec_indep_input_acts_eq ‹_› ‹_›
+    refine ⟨?_, by simp [exec]⟩
+    ext1
+    exact exec_indep_restriction_eq hn hi m₁ m₂
     
-    /-
-theorem InstStep.indep_rcns_indep_output :
-  (e : s ⇓ᵢ s') → (rcn' <[s.rtr]> e.rcn) → (rcn' ≠ e.rcn) → s.output rcn' = s'.rcnOutput rcn' := by
-  intro h hi hrne
-  have hp := h.exec.preserves_rcns
-  cases ho : s.rtr[.rcn][rcn'] <;> cases ho' : s'.rtr[.rcn][rcn']
-  case none.none => simp [State.rcnOutput, ho, ho']
-  case' none.some, some.none => simp [hp, ho'] at ho
-  case some.some => 
-    have ⟨⟨p, a, x, t⟩, hj⟩ := State.rcnInput_iff_obj?.mpr ⟨_, ho⟩
-    have ⟨⟨p', a', x', t'⟩, hj'⟩ := State.rcnInput_iff_obj?.mpr ⟨_, ho'⟩
-    have H1 : p = p' := by 
-      simp [s.rcnInput_ports_def hj ho, s'.rcnInput_ports_def hj' ho']
-      rw [←hp] at ho'
-      have he := Option.some_inj.mp $ ho.symm.trans ho'
-      simp [he]
-      sorry
-    sorry
-      
-      refine congr_arg₂ _ ?_ rfl
-      apply Finmap.restrict_ext
-      intro p hp
-      have ⟨_, hr⟩ := Reactor.contains_iff_obj?.mp h.rtr_contains_rcn
-      have hd := hi.symm.nonoverlapping_deps hr ho'
-      simp [Finset.eq_empty_iff_forall_not_mem, Finset.mem_inter] at hd
-      have hd := mt (hd p) $ not_not.mpr hp
-      simp [Reactor.obj?'_eq_obj?, h.preserves_nondep_ports hr hd]
-    have H2 : a = a' := by
-      simp [s.rcnInput_actions_def hj ho, s'.rcnInput_actions_def hj' ho']
-      rw [←hp] at ho'
-      have he := Option.some_inj.mp $ ho.symm.trans ho'
-      simp [he]
-      apply Finmap.restrict_ext
-      intro a ha
-      simp [h.preserves_tag]
-      apply Finmap.filterMap_congr
-      have ⟨_, hr⟩ := Reactor.contains_iff_obj?.mp h.rtr_contains_rcn
-      have hd := hi.symm.nonoverlapping_deps hr ho'
-      simp [Finset.eq_empty_iff_forall_not_mem, Finset.mem_inter] at hd
-      have hd := mt (hd a) $ not_not.mpr ha
-      simp [Reactor.obj?'_eq_obj?, h.preserves_nondep_actions hr hd]
-    have H3 : t = t' := by 
-      simp [s.rcnInput_time_def hj, s'.rcnInput_time_def hj', h.exec.preserves_tag]
-    simp [H1, H2, H3] at hj
-    have ⟨r, hr⟩ := Reactor.contains_iff_obj?.mp h.rtr_contains_rcn
-    have ⟨_, hc, _⟩ := Reactor.obj?_to_con?_and_cpt? ho
-    have ⟨_, hr', _⟩ := Reactor.obj?_to_con?_and_cpt? hr
-    cases hi.ne_rtr_or_pure hrne ho hr hc hr'
-    case inl he => 
-      have ⟨_, hc', _⟩ := Reactor.obj?_to_con?_and_cpt? ho'
-      have hs := State.rcnInput_state_def hj hc
-      have hs' := State.rcnInput_state_def hj' hc'
-      have hq := h.exec.equiv
-      have hh := hq.con?_id_eq hc hc'
-      have hc := Reactor.con?_to_rtr_obj? hc
-      have hc' := Reactor.con?_to_rtr_obj? hc'
-      rw [←hh] at hc'
-      rw [h.preserves_external_state hr' hc hc' he.symm] at hs
-      rw [hs.trans hs'.symm] at hj
-      exact State.rcnOutput_congr (hj.trans hj'.symm) hp
-    case inr hc =>
-      cases hc
-      case inl hp' => 
-        rw [ho'.symm.trans (h.exec.preserves_rcns ▸ ho)] at ho'
-        exact State.rcnOutput_pure_congr hj hj' ho ho' hp'
-      case inr hp' => 
-        have ⟨_, hco, _⟩ := Reactor.obj?_to_con?_and_cpt? ho
-        have ⟨_, hco', _⟩ := Reactor.obj?_to_con?_and_cpt? ho'
-        have hs := State.rcnInput_state_def hj hco
-        have hs' := State.rcnInput_state_def hj' hco'
-        suffices h : x = x' by 
-          rw [h] at hj
-          exact State.rcnOutput_congr (hj.trans hj'.symm) hp
-        rw [hs, hs']
-        have he := h.exec.equiv
-        exact (he.con?_obj_equiv hco hco').obj?_ext (cpt := .stv) (by
-          intro j _
-          have h := h.pure_preserves_state (j := j) hr hp'
-          have hh := he.con?_id_eq hco hco'
-          have hco := Reactor.con?_to_rtr_obj? hco
-          have hco' := Reactor.con?_to_rtr_obj? hco'
-          rw [←hh] at hco'
-          exact he.eq_obj?_nest h hco hco' 
-        )
-    -/
-
 namespace State
 namespace Execution
