src/ReactorModel/Objects/Reactor/ReactorType/Wellformed.lean
@@ -114,12 +114,12 @@ variable [ReactorType α] [ReactorType β] [LawfulCoe α β] {rtr : α} in secti
 -- `ValidDependency rtr .norm .in (.action i)` states that normal reactions can specify the action 
 -- identified by `i` as source.
 inductive ValidDependency (rtr : α) : Reaction.Kind → Kind → Reaction.Dependency → Prop
-  | act       : (i ∈ acts rtr) → ValidDependency rtr _ _ (.action i)
-  | prt       : (i ∈ ports rtr dk) → ValidDependency rtr _ dk (.port k i)
+  | act       : (i ∈ acts rtr) → ValidDependency rtr _ _ ⟨.act, i⟩ 
+  | prt       : (i ∈ ports rtr dk) → ValidDependency rtr _ dk ⟨.prt k, i⟩  
   | nestedIn  : (nest rtr j = some con) → (i ∈ ports con .in) → 
-                ValidDependency rtr _ .out (.port .in i)
+                ValidDependency rtr _ .out ⟨.prt .in, i⟩
   | nestedOut : (nest rtr j = some con) → (i ∈ ports con .out) → 
-                ValidDependency rtr .norm .in (.port .in i)
+                ValidDependency rtr .norm .in ⟨.prt .in, i⟩ 
 
 set_option hygiene false in
 scoped macro "lift_nested_proof " name:ident : term => `(
@@ -164,8 +164,10 @@ theorem ValidDependency.equiv
 -- TODO: Refactor the `prio` conditions into one.
 structure _root_.ReactorType.Wellformed (rtr : α) : Prop where
   uniqueInputs : (rtr[.rcn][i₁] = some rcn₁) → (rtr[.rcn][i₂] = some rcn₂) → (i₁ ≠ i₂) → 
-                 (i ∈ rtr[.prt .in]) → (.port .in i ∈ rcn₁.deps .out) → 
-                (.port .in i ∉ rcn₂.deps .out)  
+                 (i ∈ rtr[.prt .in]) → (⟨.prt .in, i⟩ ∈ rcn₁.deps .out) → 
+                 (⟨.prt .in, i⟩ ∉ rcn₂.deps .out)  
+  stateLocal   : (rtr[.rtr][i] = some con) → (rcns con j = some rcn) → 
+                 (⟨.stv, s⟩ ∈ rcn.deps k) → (s ∈ state con)
   overlapPrio  : (rtr[.rtr][i] = some con) → (rcns con i₁ = some rcn₁) → (rcns con i₂ = some rcn₂) → 
                  (i₁ ≠ i₂) → (rcn₁.deps .out ∩ rcn₂.deps .out).Nonempty → 
                  (rcn₁.prio < rcn₂.prio ∨ rcn₂.prio < rcn₁.prio)
@@ -187,11 +189,12 @@ scoped macro "wf_nested_proof " name:ident : term => `(
 )
 
 theorem nested (wf : Wellformed rtr₁) (h : nest rtr₁ i = some rtr₂) : Wellformed rtr₂ where
-  overlapPrio             := wf_nested_proof overlapPrio
-  impurePrio              := wf_nested_proof impurePrio
-  mutationPrio            := wf_nested_proof mutationPrio
-  validDeps               := wf_nested_proof validDeps
-  acyclicDeps             := wf.acyclicDeps.nested h
+  stateLocal   := wf_nested_proof stateLocal
+  overlapPrio  := wf_nested_proof overlapPrio
+  impurePrio   := wf_nested_proof impurePrio
+  mutationPrio := wf_nested_proof mutationPrio
+  validDeps    := wf_nested_proof validDeps
+  acyclicDeps  := wf.acyclicDeps.nested h
   uniqueInputs h₁ h₂ _ h₄ := 
     wf.uniqueInputs (obj?_nested h h₁) (obj?_nested h h₂) ‹_› (obj?_mem_nested h h₄)
 
@@ -207,10 +210,12 @@ theorem lift [c : LawfulCoe α β] (wf : Wellformed (rtr : β)) : Wellformed rtr
   impurePrio   := lift_prio_proof impurePrio
   mutationPrio := lift_prio_proof mutationPrio
   acyclicDeps  := wf.acyclicDeps.lift (rtr := rtr)
+  stateLocal h₁ h₂ h₃ := 
+    c.lift_mem_cpt? .stv $ wf.stateLocal (c.lower_obj?_some h₁) (c.lower_cpt?_eq_some .rcn h₂) h₃ 
   validDeps h₁ h₂ h₃ := 
     wf.validDeps (c.lower_obj?_some h₁) (c.lower_cpt?_eq_some .rcn h₂) h₃ |>.lift
-  uniqueInputs h₁ h₂ _ h₄ := 
-    wf.uniqueInputs (c.lower_obj?_some h₁) (c.lower_obj?_some h₂) ‹_› (c.lower_mem_obj? h₄)
+  uniqueInputs h₁ h₂ _ h₃ := 
+    wf.uniqueInputs (c.lower_obj?_some h₁) (c.lower_obj?_some h₂) ‹_› (c.lower_mem_obj? h₃)
 
 set_option hygiene false in
 scoped macro "equiv_prio_proof " name:ident rtr₁:ident rtr₂:ident : term => `(
@@ -226,6 +231,11 @@ theorem equiv (e : rtr₁ ≈ rtr₂) (wf : Wellformed rtr₁) : Wellformed rtr�
   impurePrio   := equiv_prio_proof impurePrio rtr₁ rtr₂
   mutationPrio := equiv_prio_proof mutationPrio rtr₁ rtr₂
   acyclicDeps  := wf.acyclicDeps.equiv e
+  stateLocal h₁ h₂ h₃ :=
+    have ⟨_, h₁'⟩ := Equivalent.obj?_some_iff e |>.mpr ⟨_, h₁⟩ 
+    have e := Equivalent.obj?_rtr_equiv e h₁' h₁
+    have h₂' := Equivalent.rcns_eq e ▸ h₂
+    Equivalent.mem_cpt?_iff e (cpt := .stv) |>.mp $ wf.stateLocal h₁' h₂' h₃
   validDeps h₁ h₂ h₃ := 
     have ⟨_, h₁'⟩ := Equivalent.obj?_some_iff e |>.mpr ⟨_, h₁⟩ 
     have e := Equivalent.obj?_rtr_equiv e h₁' h₁
